# De Morgan's Law (AND)

## Description
De Morgan's Law for AND states that the negation of a conjunction is equivalent to the disjunction of the negations. "Not (P and Q)" is the same as "(not P) or (not Q)".

## Rule Pattern
¬(P ∧ Q) ⊢ ¬P ∨ ¬Q

## Problems

### Problem 1 (Difficulty: Easy)
**Premises:**
- ¬(P ∧ Q)

**Conclusion:** ¬P ∨ ¬Q

**Brief Solution:** Apply De Morgan's Law directly.

---

### Problem 2 (Difficulty: Easy)
**Premises:**
- ¬(R ∧ S)

**Conclusion:** ¬R ∨ ¬S

**Brief Solution:** Transform the negated conjunction into a disjunction of negations.

---

### Problem 3 (Difficulty: Easy)
**Premises:**
- ¬(A ∧ B)

**Conclusion:** ¬A ∨ ¬B

**Brief Solution:** Direct application of De Morgan's Law.

---

### Problem 4 (Difficulty: Medium)
**Premises:**
- ¬((P ∨ Q) ∧ R)

**Conclusion:** ¬(P ∨ Q) ∨ ¬R

**Brief Solution:** Apply De Morgan's Law where one conjunct is a disjunction.

---

### Problem 5 (Difficulty: Medium)
**Premises:**
- ¬(P ∧ (Q ∧ R))

**Conclusion:** ¬P ∨ ¬(Q ∧ R)

**Brief Solution:** Apply De Morgan's Law to the outer conjunction.

---

### Problem 6 (Difficulty: Medium)
**Premises:**
- ¬((P → Q) ∧ R)

**Conclusion:** ¬(P → Q) ∨ ¬R

**Brief Solution:** Apply De Morgan's Law with an implication as one conjunct.

---

### Problem 7 (Difficulty: Hard)
**Premises:**
- ¬((P ∧ Q) ∧ (R ∧ S))

**Conclusion:** ¬(P ∧ Q) ∨ ¬(R ∧ S)

**Brief Solution:** Apply De Morgan's Law to a conjunction of conjunctions.

---

### Problem 8 (Difficulty: Hard)
**Premises:**
- P → Q
- ¬(P ∧ R)

**Conclusion:** ¬P ∨ ¬R

**Brief Solution:** Apply De Morgan's Law to the second premise.

---

### Problem 9 (Difficulty: Hard)
**Premises:**
- ¬(P ∧ Q)
- R

**Conclusion:** (¬P ∨ ¬Q) ∧ R

**Brief Solution:** Apply De Morgan's Law, then Conjunction with R.

---

### Problem 10 (Difficulty: Very Hard)
**Premises:**
- ¬((P ∧ Q) ∧ R)

**Conclusion:** ¬P ∨ ¬Q ∨ ¬R

**Brief Solution:** Apply De Morgan's Law twice to fully distribute the negation.