# De Morgan's Law (OR)

## Description
De Morgan's Law for OR states that the negation of a disjunction is equivalent to the conjunction of the negations. "Not (P or Q)" is the same as "(not P) and (not Q)".

## Rule Pattern
¬(P ∨ Q) ⊢ ¬P ∧ ¬Q

## Problems

### Problem 1 (Difficulty: Easy)
**Premises:**
- ¬(P ∨ Q)

**Conclusion:** ¬P ∧ ¬Q

**Brief Solution:** Apply De Morgan's Law directly.

---

### Problem 2 (Difficulty: Easy)
**Premises:**
- ¬(R ∨ S)

**Conclusion:** ¬R ∧ ¬S

**Brief Solution:** Transform the negated disjunction into a conjunction of negations.

---

### Problem 3 (Difficulty: Easy)
**Premises:**
- ¬(A ∨ B)

**Conclusion:** ¬A ∧ ¬B

**Brief Solution:** Direct application of De Morgan's Law.

---

### Problem 4 (Difficulty: Medium)
**Premises:**
- ¬((P ∧ Q) ∨ R)

**Conclusion:** ¬(P ∧ Q) ∧ ¬R

**Brief Solution:** Apply De Morgan's Law where one disjunct is a conjunction.

---

### Problem 5 (Difficulty: Medium)
**Premises:**
- ¬(P ∨ (Q ∨ R))

**Conclusion:** ¬P ∧ ¬(Q ∨ R)

**Brief Solution:** Apply De Morgan's Law to the outer disjunction.

---

### Problem 6 (Difficulty: Medium)
**Premises:**
- ¬((P → Q) ∨ R)

**Conclusion:** ¬(P → Q) ∧ ¬R

**Brief Solution:** Apply De Morgan's Law with an implication as one disjunct.

---

### Problem 7 (Difficulty: Hard)
**Premises:**
- ¬((P ∨ Q) ∨ (R ∨ S))

**Conclusion:** ¬(P ∨ Q) ∧ ¬(R ∨ S)

**Brief Solution:** Apply De Morgan's Law to a disjunction of disjunctions.

---

### Problem 8 (Difficulty: Hard)
**Premises:**
- P → Q
- ¬(P ∨ R)

**Conclusion:** ¬P ∧ ¬R

**Brief Solution:** Apply De Morgan's Law to the second premise.

---

### Problem 9 (Difficulty: Hard)
**Premises:**
- ¬(P ∨ Q)

**Conclusion:** ¬P

**Brief Solution:** Apply De Morgan's Law to get "¬P ∧ ¬Q", then Simplification to extract ¬P.

---

### Problem 10 (Difficulty: Very Hard)
**Premises:**
- ¬((P ∨ Q) ∨ R)

**Conclusion:** ¬P ∧ ¬Q ∧ ¬R

**Brief Solution:** Apply De Morgan's Law twice to fully distribute the negation.